src/Contracts/Flex/Functions/FuncNotations.v
@@ -1,0 +1,332 @@
+
+Require Import Coq.Program.Basics. 
+Require Import Coq.Strings.String. 
+Require Import ZArith.
+
+Require Import FinProof.Common.
+Require Import FinProof.ProgrammingWith.
+Require Import FinProof.MonadTransformers21.
+
+Require Import UMLang.SolidityNotations2.
+Require Import UMLang.UrsusLib.
+
+Require Import UrsusTVM.tvmFunc.
+Require Import UrsusTVM.tvmNotations.
+
+Require Import Project.CommonConstSig.
+
+Require Import Contracts.Flex.Ledger.
+Require Import Contracts.Flex.Functions.FuncSig.
+
+(* здесь инмпортируем все внешние интерфейсы *)
+Require Import Interface.
+
+Module FuncNotations (xt: XTypesSig) 
+                     (sm: StateMonadSig) 
+                     (dc : ConstsTypesSig xt sm ).
+Export dc. Export xt. Export sm.
+
+(* здесь модули из каждого внешнего интерфейса *)
+Module FlexPublicInterface := PublicInterface xt sm.
+
+Module Export SpecModuleForFuncNotations := Spec xt sm.
+
+
+Import xt.
+
+Import UrsusNotations.
+
+Local Open Scope ursus_scope.
+
+
+Notation " 'TickTock.tick' " := ( TickTock_ι_tick ) (in custom ULValue at level 0) : ursus_scope. 
+ Notation " 'TickTock.tick' " := ( TickTock_ι_tick ) (in custom URValue at level 0) : ursus_scope. 
+ Notation " 'TickTock.tock' " := ( TickTock_ι_tock ) (in custom ULValue at level 0) : ursus_scope. 
+ Notation " 'TickTock.tock' " := ( TickTock_ι_tock ) (in custom URValue at level 0) : ursus_scope. 
+ Notation " 'anycast_info.rewrite_pfx' " := ( anycast_info_ι_rewrite_pfx ) (in custom ULValue at level 0) : ursus_scope. 
+ Notation " 'anycast_info.rewrite_pfx' " := ( anycast_info_ι_rewrite_pfx ) (in custom URValue at level 0) : ursus_scope. 
+ Notation " 'addr_std.kind' " := ( addr_std_ι_kind ) (in custom ULValue at level 0) : ursus_scope. 
+ Notation " 'addr_std.kind' " := ( addr_std_ι_kind ) (in custom URValue at level 0) : ursus_scope. 
+ Notation " 'addr_std.Anycast' " := ( addr_std_ι_Anycast ) (in custom ULValue at level 0) : ursus_scope. 
+ Notation " 'addr_std.Anycast' " := ( addr_std_ι_Anycast ) (in custom URValue at level 0) : ursus_scope. 
+ Notation " 'addr_std.workchain_id' " := ( addr_std_ι_workchain_id ) (in custom ULValue at level 0) : ursus_scope. 
+ Notation " 'addr_std.workchain_id' " := ( addr_std_ι_workchain_id ) (in custom URValue at level 0) : ursus_scope. 
+ Notation " 'addr_std.address' " := ( addr_std_ι_address ) (in custom ULValue at level 0) : ursus_scope. 
+ Notation " 'addr_std.address' " := ( addr_std_ι_address ) (in custom URValue at level 0) : ursus_scope. 
+ Notation " 'TonsConfig.transfer_tip3' " := ( TonsConfig_ι_transfer_tip3 ) (in custom ULValue at level 0) : ursus_scope. 
+ Notation " 'TonsConfig.transfer_tip3' " := ( TonsConfig_ι_transfer_tip3 ) (in custom URValue at level 0) : ursus_scope. 
+ Notation " 'TonsConfig.return_ownership' " := ( TonsConfig_ι_return_ownership ) (in custom ULValue at level 0) : ursus_scope. 
+ Notation " 'TonsConfig.return_ownership' " := ( TonsConfig_ι_return_ownership ) (in custom URValue at level 0) : ursus_scope. 
+ Notation " 'TonsConfig.trading_pair_deploy' " := ( TonsConfig_ι_trading_pair_deploy ) (in custom ULValue at level 0) : ursus_scope. 
+ Notation " 'TonsConfig.trading_pair_deploy' " := ( TonsConfig_ι_trading_pair_deploy ) (in custom URValue at level 0) : ursus_scope. 
+ Notation " 'TonsConfig.order_answer' " := ( TonsConfig_ι_order_answer ) (in custom ULValue at level 0) : ursus_scope. 
+ Notation " 'TonsConfig.order_answer' " := ( TonsConfig_ι_order_answer ) (in custom URValue at level 0) : ursus_scope. 
+ Notation " 'TonsConfig.process_queue' " := ( TonsConfig_ι_process_queue ) (in custom ULValue at level 0) : ursus_scope. 
+ Notation " 'TonsConfig.process_queue' " := ( TonsConfig_ι_process_queue ) (in custom URValue at level 0) : ursus_scope. 
+ Notation " 'TonsConfig.send_notify' " := ( TonsConfig_ι_send_notify ) (in custom ULValue at level 0) : ursus_scope. 
+ Notation " 'TonsConfig.send_notify' " := ( TonsConfig_ι_send_notify ) (in custom URValue at level 0) : ursus_scope. 
+ Notation " 'FlexOwnershipInfo.deployer_pubkey' " := ( FlexOwnershipInfo_ι_deployer_pubkey ) (in custom ULValue at level 0) : ursus_scope. 
+ Notation " 'FlexOwnershipInfo.deployer_pubkey' " := ( FlexOwnershipInfo_ι_deployer_pubkey ) (in custom URValue at level 0) : ursus_scope. 
+ Notation " 'FlexOwnershipInfo.ownership_description' " := ( FlexOwnershipInfo_ι_ownership_description ) (in custom ULValue at level 0) : ursus_scope. 
+ Notation " 'FlexOwnershipInfo.ownership_description' " := ( FlexOwnershipInfo_ι_ownership_description ) (in custom URValue at level 0) : ursus_scope. 
+ Notation " 'FlexOwnershipInfo.owner_contract' " := ( FlexOwnershipInfo_ι_owner_contract ) (in custom ULValue at level 0) : ursus_scope. 
+ Notation " 'FlexOwnershipInfo.owner_contract' " := ( FlexOwnershipInfo_ι_owner_contract ) (in custom URValue at level 0) : ursus_scope. 
+ 
+ Definition deployer_pubkey__left := ( ULState (f:=_Contract) (H:=ContractLEmbeddedType deployer_pubkey_ ) : ULValue XInteger256 ) . 
+ Definition deployer_pubkey__right := ( URState (f:=_Contract) (H:=ContractLEmbeddedType deployer_pubkey_ ) : URValue XInteger256 false ) . 
+ Notation " '_deployer_pubkey_' " := ( deployer_pubkey__left ) (in custom ULValue at level 0) : ursus_scope. 
+ Notation " '_deployer_pubkey_' " := ( deployer_pubkey__right ) (in custom URValue at level 0) : ursus_scope. 
+ 
+ Definition ownership_description__left := ( ULState (f:=_Contract) (H:=ContractLEmbeddedType ownership_description_ ) : ULValue XString ) . 
+ Definition ownership_description__right := ( URState (f:=_Contract) (H:=ContractLEmbeddedType ownership_description_ ) : URValue XString false ) . 
+ Notation " '_ownership_description_' " := ( ownership_description__left ) (in custom ULValue at level 0) : ursus_scope. 
+ Notation " '_ownership_description_' " := ( ownership_description__right ) (in custom URValue at level 0) : ursus_scope. 
+ 
+ Definition owner_address__left := ( ULState (f:=_Contract) (H:=ContractLEmbeddedType owner_address_ ) : ULValue ( XMaybe XAddress ) ) . 
+ Definition owner_address__right := ( URState (f:=_Contract) (H:=ContractLEmbeddedType owner_address_ ) : URValue ( XMaybe XAddress ) false ) . 
+ Notation " '_owner_address_' " := ( owner_address__left ) (in custom ULValue at level 0) : ursus_scope. 
+ Notation " '_owner_address_' " := ( owner_address__right ) (in custom URValue at level 0) : ursus_scope. 
+ 
+ Definition tons_cfg__left := ( ULState (f:=_Contract) (H:=ContractLEmbeddedType tons_cfg_ ) : ULValue TonsConfigLRecord ) . 
+ Definition tons_cfg__right := ( URState (f:=_Contract) (H:=ContractLEmbeddedType tons_cfg_ ) : URValue TonsConfigLRecord false ) . 
+ Notation " '_tons_cfg_' " := ( tons_cfg__left ) (in custom ULValue at level 0) : ursus_scope. 
+ Notation " '_tons_cfg_' " := ( tons_cfg__right ) (in custom URValue at level 0) : ursus_scope. 
+ 
+ Definition pair_code__left := ( ULState (f:=_Contract) (H:=ContractLEmbeddedType pair_code_ ) : ULValue ( XMaybe XCell ) ) . 
+ Definition pair_code__right := ( URState (f:=_Contract) (H:=ContractLEmbeddedType pair_code_ ) : URValue ( XMaybe XCell ) false ) . 
+ Notation " '_pair_code_' " := ( pair_code__left ) (in custom ULValue at level 0) : ursus_scope. 
+ Notation " '_pair_code_' " := ( pair_code__right ) (in custom URValue at level 0) : ursus_scope. 
+ 
+ Definition xchg_pair_code__left := ( ULState (f:=_Contract) (H:=ContractLEmbeddedType xchg_pair_code_ ) : ULValue ( XMaybe XCell ) ) . 
+ Definition xchg_pair_code__right := ( URState (f:=_Contract) (H:=ContractLEmbeddedType xchg_pair_code_ ) : URValue ( XMaybe XCell ) false ) . 
+ Notation " '_xchg_pair_code_' " := ( xchg_pair_code__left ) (in custom ULValue at level 0) : ursus_scope. 
+ Notation " '_xchg_pair_code_' " := ( xchg_pair_code__right ) (in custom URValue at level 0) : ursus_scope. 
+ 
+ Definition price_code__left := ( ULState (f:=_Contract) (H:=ContractLEmbeddedType price_code_ ) : ULValue ( XMaybe XCell ) ) . 
+ Definition price_code__right := ( URState (f:=_Contract) (H:=ContractLEmbeddedType price_code_ ) : URValue ( XMaybe XCell ) false ) . 
+ Notation " '_price_code_' " := ( price_code__left ) (in custom ULValue at level 0) : ursus_scope. 
+ Notation " '_price_code_' " := ( price_code__right ) (in custom URValue at level 0) : ursus_scope. 
+ 
+ Definition xchg_price_code__left := ( ULState (f:=_Contract) (H:=ContractLEmbeddedType xchg_price_code_ ) : ULValue ( XMaybe XCell ) ) . 
+ Definition xchg_price_code__right := ( URState (f:=_Contract) (H:=ContractLEmbeddedType xchg_price_code_ ) : URValue ( XMaybe XCell ) false ) . 
+ Notation " '_xchg_price_code_' " := ( xchg_price_code__left ) (in custom ULValue at level 0) : ursus_scope. 
+ Notation " '_xchg_price_code_' " := ( xchg_price_code__right ) (in custom URValue at level 0) : ursus_scope. 
+ 
+ Definition deals_limit__left := ( ULState (f:=_Contract) (H:=ContractLEmbeddedType deals_limit_ ) : ULValue XInteger8 ) . 
+ Definition deals_limit__right := ( URState (f:=_Contract) (H:=ContractLEmbeddedType deals_limit_ ) : URValue XInteger8 false ) . 
+ Notation " '_deals_limit_' " := ( deals_limit__left ) (in custom ULValue at level 0) : ursus_scope. 
+ Notation " '_deals_limit_' " := ( deals_limit__right ) (in custom URValue at level 0) : ursus_scope. 
+ Notation " 'StateInit.split_depth' " := ( StateInit_ι_split_depth ) (in custom ULValue at level 0) : ursus_scope. 
+ Notation " 'StateInit.split_depth' " := ( StateInit_ι_split_depth ) (in custom URValue at level 0) : ursus_scope. 
+ Notation " 'StateInit.special' " := ( StateInit_ι_special ) (in custom ULValue at level 0) : ursus_scope. 
+ Notation " 'StateInit.special' " := ( StateInit_ι_special ) (in custom URValue at level 0) : ursus_scope. 
+ Notation " 'StateInit.code' " := ( StateInit_ι_code ) (in custom ULValue at level 0) : ursus_scope. 
+ Notation " 'StateInit.code' " := ( StateInit_ι_code ) (in custom URValue at level 0) : ursus_scope. 
+ Notation " 'StateInit.data' " := ( StateInit_ι_data ) (in custom ULValue at level 0) : ursus_scope. 
+ Notation " 'StateInit.data' " := ( StateInit_ι_data ) (in custom URValue at level 0) : ursus_scope. 
+ Notation " 'StateInit.library' " := ( StateInit_ι_library ) (in custom ULValue at level 0) : ursus_scope. 
+ Notation " 'StateInit.library' " := ( StateInit_ι_library ) (in custom URValue at level 0) : ursus_scope. 
+ Notation " 'DTradingPair.flex_addr_' " := ( DTradingPair_ι_flex_addr_ ) (in custom ULValue at level 0) : ursus_scope. 
+ Notation " 'DTradingPair.flex_addr_' " := ( DTradingPair_ι_flex_addr_ ) (in custom URValue at level 0) : ursus_scope. 
+ Notation " 'DTradingPair.tip3_root_' " := ( DTradingPair_ι_tip3_root_ ) (in custom ULValue at level 0) : ursus_scope. 
+ Notation " 'DTradingPair.tip3_root_' " := ( DTradingPair_ι_tip3_root_ ) (in custom URValue at level 0) : ursus_scope. 
+ Notation " 'DTradingPair.deploy_value_' " := ( DTradingPair_ι_deploy_value_ ) (in custom ULValue at level 0) : ursus_scope. 
+ Notation " 'DTradingPair.deploy_value_' " := ( DTradingPair_ι_deploy_value_ ) (in custom URValue at level 0) : ursus_scope. 
+ Notation " 'DXchgPair.flex_addr_' " := ( DXchgPair_ι_flex_addr_ ) (in custom ULValue at level 0) : ursus_scope. 
+ Notation " 'DXchgPair.flex_addr_' " := ( DXchgPair_ι_flex_addr_ ) (in custom URValue at level 0) : ursus_scope. 
+ Notation " 'DXchgPair.tip3_major_root_' " := ( DXchgPair_ι_tip3_major_root_ ) (in custom ULValue at level 0) : ursus_scope. 
+ Notation " 'DXchgPair.tip3_major_root_' " := ( DXchgPair_ι_tip3_major_root_ ) (in custom URValue at level 0) : ursus_scope. 
+ Notation " 'DXchgPair.tip3_minor_root_' " := ( DXchgPair_ι_tip3_minor_root_ ) (in custom ULValue at level 0) : ursus_scope. 
+ Notation " 'DXchgPair.tip3_minor_root_' " := ( DXchgPair_ι_tip3_minor_root_ ) (in custom URValue at level 0) : ursus_scope. 
+ Notation " 'DXchgPair.deploy_value_' " := ( DXchgPair_ι_deploy_value_ ) (in custom ULValue at level 0) : ursus_scope. 
+ Notation " 'DXchgPair.deploy_value_' " := ( DXchgPair_ι_deploy_value_ ) (in custom URValue at level 0) : ursus_scope. 
+ 
+Module Calls (tc : SpecSig).
+
+Export tc.
+
+Local Open Scope string_scope.
+
+
+Definition constructor_left {R b0 b1 b2 b3 b4 b5 b6 b7 b8 b9 }
+( deployer_pubkey : URValue XInteger256 b0) 
+( ownership_description : URValue XString b1) 
+( owner_address : URValue (XMaybe XAddress) b2)
+( transfer_tip3 : URValue XInteger128 b3) 
+( return_ownership : URValue XInteger128 b4) 
+( trading_pair_deploy : URValue XInteger128 b5) 
+( order_answer : URValue XInteger128 b6)
+( process_queue : URValue XInteger8 b7) 
+( send_notify : URValue XAddress b8)
+( deals_limit : URValue XAddress b9) :  UExpression R 
+((orb(orb(orb(orb(orb(orb(orb(orb(orb b9 b8)b7)b6)b5)b4)b3)b2)b1)b0)) :=
+
+wrapULExpression (ursus_call_with_args (LedgerableWithArgs:=λ10) 
+constructor 
+deployer_pubkey
+ownership_description
+owner_address
+transfer_tip3 
+return_ownership 
+trading_pair_deploy 
+order_answer
+process_queue 
+send_notify
+deals_limit ).
+
+Notation " 'constructor_' '(' x0 ',' x1 ',' x2 ',' x3 ',' x4 ',' x5 ',' x6 ',' x7 ',' x8 ',' x9 ')' " :=
+( constructor_left x0 x1 x2 x3 x4 x5 x6 x7 x8 x9 )
+(in custom ULValue at level 0 , 
+x0 custom URValue at level 0,
+x1 custom URValue at level 0,
+x2 custom URValue at level 0,
+x3 custom URValue at level 0,
+x4 custom URValue at level 0,
+x5 custom URValue at level 0,
+x6 custom URValue at level 0,
+x7 custom URValue at level 0,
+x8 custom URValue at level 0,
+x9 custom URValue at level 0) : ursus_scope.
+
+Definition setPairCode_left {R b1} (x: URValue XCell b1 ) : UExpression R true :=
+   wrapULExpression (ursus_call_with_args (LedgerableWithArgs:=λ1) setPairCode x).    
+
+Notation " 'setPairCode_' '(' x ')' " := (setPairCode_left x)  
+   (in custom ULValue at level 0 , x custom URValue at level 0) : ursus_scope.
+
+Definition setXchgPairCode_left {R b1} (x: URValue XCell b1 ) : UExpression R true :=
+   wrapULExpression (ursus_call_with_args (LedgerableWithArgs:=λ1) setXchgPairCode x).    
+
+Notation " 'setXchgPairCode_' '(' x ')' " := (setXchgPairCode x)  
+   (in custom ULValue at level 0 , x custom URValue at level 0) : ursus_scope.
+
+Definition setPriceCode_left {R b1} (x: URValue XCell b1 ) : UExpression R true :=
+   wrapULExpression (ursus_call_with_args (LedgerableWithArgs:=λ1) setPriceCode x).    
+
+Notation " 'setPriceCode_' '(' x ')' " := (setPriceCode_left x)  
+   (in custom ULValue at level 0 , x custom URValue at level 0) : ursus_scope.
+
+Definition setXchgPriceCode_left {R b1} (x: URValue XCell b1 ) : UExpression R true :=
+   wrapULExpression (ursus_call_with_args (LedgerableWithArgs:=λ1) setXchgPriceCode x).    
+
+Notation " 'setXchgPriceCode_' '(' x ')' " := (setXchgPriceCode_left x)  
+   (in custom ULValue at level 0 , x custom URValue at level 0) : ursus_scope.
+
+Definition transfer_INTERNAL_left {R b1 b2} 
+(x0: URValue XAddress b1 ) 
+(x1: URValue XInteger128 b2 )
+: UExpression R true :=
+   wrapULExpression (ursus_call_with_args (LedgerableWithArgs:=λ2) transfer_INTERNAL x0 x1 ).    
+
+Notation " 'transfer_INTERNAL_' '(' x0 ',' x1 ')' " := (transfer_INTERNAL_left x0 x1 )  
+   (in custom ULValue at level 0 , 
+x0 custom URValue at level 0 ,
+x1 custom URValue at level 0) : ursus_scope.
+
+Definition transfer_EXTERNAL_left {R b1 b2} 
+(x0: URValue XAddress b1 ) 
+(x1: URValue XInteger128 b2 )
+: UExpression R true :=
+   wrapULExpression (ursus_call_with_args (LedgerableWithArgs:=λ2) transfer_EXTERNAL x0 x1 ).    
+
+Notation " 'transfer_EXTERNAL_' '(' x0 ',' x1 ')' " := (transfer_EXTERNAL_left x0 x1 )  
+   (in custom ULValue at level 0 , 
+x0 custom URValue at level 0 ,
+x1 custom URValue at level 0) : ursus_scope.
+
+Definition isFullyInitialized_right : URValue XBool false :=
+   wrapURExpression (ursus_call_with_args (LedgerableWithArgs:=λ0) isFullyInitialized ).    
+
+Notation " 'isFullyInitialized_' '(' ')' " := (isFullyInitialized_right )  
+   (in custom URValue at level 0 ) : ursus_scope.
+
+Definition getTonsCfg_right : URValue TonsConfigLRecord false :=
+   wrapURExpression (ursus_call_with_args (LedgerableWithArgs:=λ0) getTonsCfg ).    
+
+Notation " 'getTonsCfg_' '(' ')' " := ( getTonsCfg_right )  
+   (in custom URValue at level 0 ) : ursus_scope.
+
+Definition getTradingPairCode_right : URValue XCell false := (*TODO: maybe true*)
+   wrapURExpression (ursus_call_with_args (LedgerableWithArgs:=λ0) getTradingPairCode ).    
+
+Notation " 'getTradingPairCode_' '(' ')' " := ( getTradingPairCode_right )  
+   (in custom URValue at level 0 ) : ursus_scope.
+
+Definition getXchgPairCode_right : URValue XCell false := (*TODO: maybe true*)
+   wrapURExpression (ursus_call_with_args (LedgerableWithArgs:=λ0) getXchgPairCode ).    
+
+Notation " 'getXchgPairCode_' '(' ')' " := ( getXchgPairCode_right )  
+   (in custom URValue at level 0 ) : ursus_scope.
+
+Definition getSellPriceCode_right {b1} (x: URValue XAddress b1 ) : URValue XCell true :=
+   wrapURExpression (ursus_call_with_args (LedgerableWithArgs:=λ1) getSellPriceCode x).    
+
+Notation " 'getSellPriceCode_' '(' x ')' " := (getSellPriceCode_right x)  
+   (in custom URValue at level 0 , x custom URValue at level 0) : ursus_scope.
+
+Definition getXchgPriceCode_right {b1 b2} 
+(x0: URValue XAddress b1 ) 
+(x1: URValue XAddress b2 ) 
+: URValue XCell true :=
+   wrapURExpression (ursus_call_with_args (LedgerableWithArgs:=λ2) getXchgPriceCode x0 x1).    
+
+Notation " 'getXchgPriceCode_' '(' x0 ',' x1 ')' " := (getXchgPriceCode_right x0 x1)  
+   (in custom URValue at level 0 , 
+    x0 custom URValue at level 0,
+    x1 custom URValue at level 0) : ursus_scope.
+
+Definition getSellTradingPair_right {b1} (x: URValue XAddress b1 ) : URValue XAddress b1 :=
+   wrapURExpression (ursus_call_with_args (LedgerableWithArgs:=λ1) getSellTradingPair x).    
+
+Notation " 'getSellTradingPair_' '(' x ')' " := (getSellTradingPair_right x)  
+   (in custom URValue at level 0 , x custom URValue at level 0) : ursus_scope.
+
+Definition getXchgTradingPair_right {b1 b2} 
+(x0: URValue XAddress b1 ) 
+(x1: URValue XAddress b2 ) 
+: URValue XAddress (orb b2 b1) :=
+   wrapURExpression (ursus_call_with_args (LedgerableWithArgs:=λ2) getXchgTradingPair x0 x1).    
+
+Notation " 'getXchgTradingPair_' '(' x0 ',' x1 ')' " := (getXchgTradingPair_right x0 x1)  
+   (in custom URValue at level 0 , 
+    x0 custom URValue at level 0,
+    x1 custom URValue at level 0) : ursus_scope.
+
+Definition getDealsLimit_right : URValue XInteger8 false := 
+   wrapURExpression (ursus_call_with_args (LedgerableWithArgs:=λ0) getDealsLimit ).    
+
+Notation " 'getDealsLimit_' '(' ')' " := ( getDealsLimit_right )  
+   (in custom URValue at level 0 ) : ursus_scope.
+
+Definition getOwnershipInfo_right : URValue FlexOwnershipInfoLRecord false := 
+   wrapURExpression (ursus_call_with_args (LedgerableWithArgs:=λ0) getOwnershipInfo ).    
+
+Notation " 'getOwnershipInfo_' '(' ')' " := ( getOwnershipInfo_right )  
+   (in custom URValue at level 0 ) : ursus_scope.
+
+Definition _fallback_right {b1 b2} 
+(x0: URValue XCell b1 ) 
+(x1: URValue XSlice b2 ) 
+: URValue XInteger (orb b2 b1) :=
+   wrapURExpression (ursus_call_with_args (LedgerableWithArgs:=λ2) _fallback x0 x1).    
+
+Notation " '_fallback_' '(' x0 ',' x1 ')' " := (_fallback_right x0 x1)  
+   (in custom URValue at level 0 , 
+    x0 custom URValue at level 0,
+    x1 custom URValue at level 0) : ursus_scope.
+
+Definition prepare_flex_state_init_and_addr_right {b1 b2} 
+(x0: URValue ContractLRecord b1 ) 
+(x1: URValue XCell b2 ) 
+: URValue ( StateInitLRecord # XInteger256 )%sol (orb b2 b1) :=
+   wrapURExpression (ursus_call_with_args (LedgerableWithArgs:=λ2) prepare_flex_state_init_and_addr x0 x1).    
+
+Notation " 'prepare_flex_state_init_and_addr_' '(' x0 ',' x1 ')' " := (prepare_flex_state_init_and_addr_right x0 x1)  
+   (in custom URValue at level 0 , 
+    x0 custom URValue at level 0,
+    x1 custom URValue at level 0) : ursus_scope.
+
+
+End Calls. 
+
+End FuncNotations.
