src/Contracts/Flex/Functions/FuncSig.v
@@ -1,3 +1,5 @@
+Require Import FinProof.Common. 
+
 Require Import UMLang.SolidityNotations2.
 Require Import UMLang.UrsusLib.
 Require Import UrsusTVM.tvmNotations.
@@ -13,16 +15,17 @@ Module Export tvmNotationsModule := tvmNotations xt sm LedgerModuleForFuncSig.
 
 Module Type SpecSig.
 
-Parameter constructor1 : URValue XInteger256 false -> URValue XString false -> URValue ( XMaybe XAddress) false -> URValue XInteger128 false -> URValue XInteger128 false -> URValue XInteger128 false -> URValue XInteger128 false -> URValue XInteger128 false -> URValue XInteger128 false -> URValue XInteger8 false -> UExpression PhantomType false . 
+Parameter constructor : URValue XInteger256 false -> URValue XString false -> URValue ( XMaybe XAddress) false -> URValue XInteger128 false -> URValue XInteger128 false -> URValue XInteger128 false -> URValue XInteger128 false -> URValue XInteger128 false -> URValue XInteger128 false -> URValue XInteger8 false -> UExpression PhantomType false . 
  Parameter setPairCode : URValue XCell false -> UExpression PhantomType true . 
  Parameter setXchgPairCode : URValue XCell false -> UExpression PhantomType true . 
  Parameter setPriceCode : URValue XCell false -> UExpression PhantomType true . 
  Parameter setXchgPriceCode : URValue XCell false -> UExpression PhantomType true . 
- Parameter transfer : URValue XAddress false -> URValue XInteger128 false -> UExpression PhantomType true . 
+ Parameter transfer_INTERNAL : URValue XAddress false -> URValue XInteger128 false -> UExpression PhantomType true . 
+ Parameter transfer_EXTERNAL : URValue XAddress false -> URValue XInteger128 false -> UExpression PhantomType true . 
  Parameter isFullyInitialized : UExpression XBool false . 
  Parameter getTonsCfg : UExpression TonsConfigLRecord false . 
- Parameter getTradingPairCode : UExpression XCell false . 
- Parameter getXchgPairCode : UExpression XCell false . 
+ Parameter getTradingPairCode : UExpression XCell false . (*TODO: maybe true*)
+ Parameter getXchgPairCode : UExpression XCell false . (*TODO: maybe true*)
  Parameter getSellPriceCode : URValue XAddress false -> UExpression XCell true . 
  Parameter getXchgPriceCode : URValue XAddress false -> URValue XAddress false -> UExpression XCell true . 
  Parameter getSellTradingPair : URValue XAddress false -> UExpression XAddress false . 
@@ -32,9 +35,9 @@ Parameter constructor1 : URValue XInteger256 false -> URValue XString false -> U
  Parameter _fallback : URValue XCell false -> URValue XSlice false -> UExpression XInteger false . 
  Parameter prepare_flex_state_init_and_addr : URValue ContractLRecord false -> URValue XCell false -> UExpression ( StateInitLRecord # XInteger256 )%sol false . 
 
-Locate constructor1.
+
 End SpecSig.
-Locate constructor1.
+
 End Spec.  
 
 
